Clean up Helper
Move relevant functions to NatArith.dfy and RealArith.dfy and remove unused ones.

src/Math/NatArith.dfy
@@ -7,6 +7,33 @@ module NatArith {
     if a < b then a else b
   }
 
+  function Power(b: nat, n: nat): (p: nat)
+    ensures b > 0 ==> p > 0
+  {
+    match n
+    case 0 => 1
+    case 1 => b
+    case _ => b * Power(b, n - 1)
+  }
+
+  function Log2Floor(n: nat): nat
+    requires n >= 1
+    decreases n
+  {
+    if n < 2
+    then 0
+    else Log2Floor(n / 2) + 1
+  }
+
+  lemma Log2FloorDef(n: nat)
+    requires n >= 1
+    ensures Log2Floor(2 * n) == Log2Floor(n) + 1
+  {}
+
+  function boolToNat(b: bool): nat {
+    if b then 1 else 0
+  }
+
   // Computes the rising factorial start^(n),
   // i.e. the product `start * (start + 1) * ... * (start + n - 1)`, i.e. with n factors.
   // see: https://en.wikipedia.org/wiki/Falling_and_rising_factorials
@@ -23,5 +50,40 @@ module NatArith {
     reveal Factorial();
   }
 
-  // TODO: a lot of functions from the helper module should go here.
+  lemma PowerGreater0(base: nat, exponent: nat)
+    requires base >= 1
+    ensures Power(base, exponent) >= 1
+  {}
+
+  lemma Power2OfLog2Floor(n: nat)
+    requires n >= 1
+    ensures Power(2, Log2Floor(n)) <= n < Power(2, Log2Floor(n) + 1)
+  {}
+
+  lemma NLtPower2Log2FloorOf2N(n: nat)
+    requires n >= 1
+    ensures n < Power(2, Log2Floor(2 * n))
+  {
+    calc {
+      n;
+    < { Power2OfLog2Floor(n); }
+      Power(2, Log2Floor(n) + 1);
+    == { Log2FloorDef(n); }
+      Power(2, Log2Floor(2 * n));
+    }
+  }
+
+  lemma MulMonotonic(a: nat, b: nat, c: nat, d: nat)
+    requires a <= c
+    requires b <= d
+    ensures a * b <= c * d
+  {
+    calc {
+      a * b;
+    <=
+      c * b;
+    <=
+      c * d;
+    }
+  }
 }
